src/Lean/Meta/Sym/DSimp/EvalGround.lean
@@ -532,6 +532,7 @@ public def evalGround (config : EvalStepConfig := {}) : DSimproc := fun e =>
   | Nat.gcd a b => evalBinNat Nat.gcd a b
   | Nat.succ a => evalUnaryNat (· + 1) a
   | Nat.log2 a => evalLog2 a config.maxExponent
+  | Nat.popcount a => evalUnaryNat Nat.popcount a
   | Int.gcd a b => evalIntGcd a b
   | Int.tdiv a b => evalBinInt Int.tdiv a b
   | Int.fdiv a b => evalBinInt Int.fdiv a b
